specs/lemmas/Spec.Blake2.Incremental.fsti
@@ -10,7 +10,7 @@ val blake2_is_hash_incremental
   (a : blake_alg)
   (input : bytes {S.length input `less_than_max_input_length` a}) :
   Lemma (
-    S.equal (Spec.Blake2.blake2 (to_blake_alg a) input
+    S.equal (Spec.Blake2.blake2 (to_blake_alg a) false input
               (Spec.Blake2.blake2_default_params (to_blake_alg a))
               Seq.empty)
             (hash_incremental a input ()))
